Finish the iterator example

theories/iterator.v
@@ -49,6 +49,10 @@ Definition iterator_trace t :=
                ∀ (k:nat), j < k < i → t !! k ≠ Some ("add", #()) ∧
                                       t !! k ≠ Some ("remove", #()).
 
+Lemma iterator_trace_nil :
+  iterator_trace [].
+Proof. unfold iterator_trace. go*. Qed.
+
 Lemma iterator_trace_size t :
   iterator_trace t →
   iterator_trace (t ++ [("size", #())]).
@@ -63,6 +67,25 @@ Lemma iterator_trace_remove t :
   iterator_trace t →
   iterator_trace (t ++ [("remove", #())]).
 Proof. unfold iterator_trace. go*. Qed.
+
+Lemma iterator_trace_iterator t x :
+  iterator_trace t →
+  iterator_trace (t ++ [("iterator", x)]).
+Proof. unfold iterator_trace. go*. Qed.
+
+Lemma iterator_trace_next t t' (n0 k: nat) x :
+  t' !! k = Some ("iterator", x) →
+  t' `prefix_of` t →
+  n0 ≤ k →
+  (∀ (k:nat) lbl,
+     n0 ≤ k → t !! k = Some (lbl, #()) → lbl ≠ "add" ∧ lbl ≠ "remove") →
+  iterator_trace t →
+  iterator_trace (t ++ [("next", x)]).
+Proof.
+  intros ? ? ? Har Ht ? ? ?. go.
+  { unfold iterator_trace in Ht. clear Har. go*. }
+  { eexists. repeat split. all: go. go. }
+Qed.
 
 End Trace.
 
@@ -94,19 +117,19 @@ Definition next : val :=
 Definition Coll (x: val) : iProp Σ :=
   ∃ (y:val) (n: nat), ⌜x = (y, # n)%V⌝ ∗ Coll_impl y ∗
   ∃ t, trace_is t ∗ trace_inv N iterator_trace ∗
-       (* ⌜n ≤ length t⌝ ∗ *)
-       ⌜∀ (k:nat) lbl, n < k → t !! k = Some (lbl, #()) →
+       ⌜n ≤ length t⌝ ∗
+       ⌜∀ (k:nat) lbl, n ≤ k → t !! k = Some (lbl, #()) →
                        lbl ≠ "add" ∧ lbl ≠ "remove"⌝.
 
 Definition Iter (r x: val) : iProp Σ :=
   ∃ (y:val) (n: nat), ⌜x = (y, # n)%V⌝ ∗ Iter_impl r y ∗
-  ∃ t, hist t ∗ ⌜∃ (k:nat), n < k ∧ t !! k = Some ("iterator", r)⌝.
+  ∃ t, hist t ∗ ⌜∃ (k:nat), n ≤ k ∧ t !! k = Some ("iterator", r)⌝.
 
 Lemma size_correct :
   size_spec Coll_impl Iter_impl size_impl -∗
   size_spec Coll Iter size.
 Proof.
-  iIntros "#spec". iIntros (c) "!>". iIntros (φ) "Hc Hφ".
+  iIntros "#spec". iIntros (c φ) "!> Hc Hφ".
   unfold size. wp_pures. wp_bind (size_impl _).
   iDestruct "Hc" as (? ? ?) "(? & Ht)". iDestruct "Ht" as (t) "(Ht & #HI & %)".
   iMod (trace_is_inv with "Ht HI") as "(Ht & %)".
@@ -114,14 +137,14 @@ Proof.
   wp_bind (Emit _ _). iApply (wp_emit with "[$Ht $HI]"); eauto.
   by apply iterator_trace_size.
   iIntros "!> Ht". wp_pures. iApply "Hφ". unfold Coll.
-  iExists _, _. iFrame. iSplitR; eauto. iExists _. iFrame "HI ∗". iPureIntro. go.
+  iExists _, _. iFrame. iSplitR; eauto. iExists _. iFrame "HI ∗". iPureIntro. go*.
 Qed.
 
 Lemma add_correct :
   add_spec Coll_impl Iter_impl add_impl -∗
   add_spec Coll Iter add.
 Proof.
-  iIntros "#spec". iIntros (c x) "!>". iIntros (φ) "Hc Hφ".
+  iIntros "#spec". iIntros (c x φ) "!> Hc Hφ".
   unfold add. wp_pures. wp_bind (add_impl _).
   iDestruct "Hc" as (? ? ?) "(? & Ht)". iDestruct "Ht" as (t) "(Ht & #HI & _)".
   iMod (trace_is_inv with "Ht HI") as "(Ht & %)".
@@ -129,14 +152,14 @@ Proof.
   iApply (wp_emit with "[$Ht $HI]"); eauto.
   by apply iterator_trace_add.
   iIntros "!> Ht". iApply ("Hφ" $! (_, # (length t + 1)%nat)%V). unfold Coll.
-  iExists _, _. iFrame. iSplitR; eauto. iExists _. iFrame "HI ∗". iPureIntro. go.
+  iExists _, _. iFrame. iSplitR; eauto. iExists _. iFrame "HI ∗". iPureIntro. go*.
 Qed.
 
 Lemma remove_correct :
   remove_spec Coll_impl Iter_impl remove_impl -∗
   remove_spec Coll Iter remove.
 Proof.
-  iIntros "#spec". iIntros (c x) "!>". iIntros (φ) "Hc Hφ".
+  iIntros "#spec". iIntros (c x φ) "!> Hc Hφ".
   unfold remove. wp_pures. wp_bind (remove_impl _).
   iDestruct "Hc" as (? ? ?) "(? & Ht)". iDestruct "Ht" as (t) "(Ht & #HI & _)".
   iMod (trace_is_inv with "Ht HI") as "(Ht & %)".
@@ -144,5 +167,96 @@ Proof.
   iApply (wp_emit with "[$Ht $HI]"); eauto.
   by apply iterator_trace_remove.
   iIntros "!> Ht". iApply ("Hφ" $! (_, # (length t + 1)%nat)%V). unfold Coll.
-  iExists _, _. iFrame. iSplitR; eauto. iExists _. iFrame "HI ∗". iPureIntro. go.
+  iExists _, _. iFrame. iSplitR; eauto. iExists _. iFrame "HI ∗". iPureIntro. go*.
+Qed.
+
+Lemma iterator_correct :
+  iterator_spec Coll_impl Iter_impl iterator_impl -∗
+  iterator_spec Coll Iter iterator.
+Proof.
+  iIntros "#spec". iIntros (c φ) "!> Hc Hφ".
+  unfold iterator. wp_pures. wp_bind (iterator_impl _).
+  iDestruct "Hc" as (? ? ?) "(? & Ht)". iDestruct "Ht" as (t) "(Ht & #HI & [% %])".
+  iMod (trace_is_inv with "Ht HI") as "(Ht & %)".
+  iApply ("spec" with "[$]"). iIntros "!>" (?) "(Hc & Hi)". wp_pures.
+  wp_bind (Emit _ _). iApply (wp_emit with "[$Ht $HI]"); eauto.
+  by apply iterator_trace_iterator.
+  iIntros "!> Ht". wp_pures.
+  iDestruct (alloc_hist with "Ht") as "(Ht & Hh)".
+  iApply "Hφ". iSplitL "Hc Ht".
+  { iExists _, _. iFrame. iSplitR; eauto. iExists _. iFrame "HI ∗". iPureIntro. go*. }
+  { iExists _, _. iFrame. iSplitR; eauto. iExists _. iFrame. iPureIntro.
+    exists (length t). go*. }
+Qed.
+
+Lemma next_correct :
+  next_spec Coll_impl Iter_impl next_impl -∗
+  next_spec Coll Iter next.
+Proof.
+  iIntros "#spec". iIntros (c x φ) "!> (Hc & Hi) Hφ".
+  unfold next. wp_pures. wp_bind (next_impl _).
+  iDestruct "Hc" as (? ? ?) "(? & Ht)".
+  iDestruct "Ht" as (t) "(Ht & #HI & [% %])".
+  iDestruct "Hi" as (? ? ?) "(? & Ht')".
+  iDestruct "Ht'" as (t') "(Ht' & %)".
+  simplify_eq.
+  iDestruct (hist_trace_is_prefix with "Ht Ht'") as %?.
+  iMod (trace_is_inv with "Ht HI") as "(Ht & %)".
+  iApply ("spec" with "[$]"). iIntros "!> (Hc & Hi)". wp_pures.
+  wp_bind (Emit _ _). iApply (wp_emit with "[$Ht $HI]"); eauto.
+  { go. by eapply iterator_trace_next. }
+  iIntros "!> Ht". wp_pures.
+  iDestruct (alloc_hist with "Ht") as "(Ht & Hh)".
+  iApply "Hφ". iSplitL "Hc Ht".
+  { iExists _, _. iFrame. iSplitR; eauto. iExists _. iFrame "HI ∗". iPureIntro. go*. }
+  { iExists _, _. iFrame. iSplitR; eauto. iExists _. iFrame. iPureIntro. go*. }
+Qed.
+
+End S.
+
+Definition lib (lib_impl: val): val :=
+  match lib_impl with
+  | (size_impl, add_impl, remove_impl, iterator_impl, next_impl)%V =>
+    (size size_impl, add add_impl, remove remove_impl, iterator iterator_impl, next next_impl)
+  | _ => #()
+  end.
+
+Lemma correct `{!heapG Σ} N P0 (lib_impl: val) :
+  iterlib_spec P0 lib_impl -∗
+  iterlib_spec (P0 ∗ trace_is [] ∗ trace_inv N iterator_trace) (lib lib_impl).
+Proof.
+  iIntros "#S". iDestruct "S" as (Coll_impl Iter_impl) "(#H0 & S)".
+  repeat case_match; eauto. iDestruct "S" as "(? & ? & ? & ? & ?)".
+  subst. unfold iterlib_spec.
+  iExists (Coll N Coll_impl), (Iter Iter_impl). repeat iSplit.
+  { iIntros "!> (HP0 & ? & ?)". iDestruct ("H0" with "HP0") as (c) "?".
+    iExists _. unfold Coll. iExists c, 0%nat. iSplitR; eauto.
+    iFrame. iExists []. iFrame. iPureIntro. go*. }
+  iApply size_correct; eauto.
+  iApply add_correct; eauto.
+  iApply remove_correct; eauto.
+  iApply iterator_correct; eauto.
+  iApply next_correct; eauto.
+Qed.
+
+End Wrap.
+
+Definition iterlibN := nroot .@ "iterlib".
+Definition empty_state : state := Build_state ∅ [] ∅.
+
+Lemma wrap_iterlib_correct {Σ} `{heapPreG Σ} (e: val → expr) (lib: val):
+  (⊢ ∀ `{heapG Σ}, iterlib_spec True lib) →
+  (⊢ ∀ `{heapG Σ} P lib, iterlib_spec P lib -∗ {{{ P }}} e lib {{{ v, RET v; True }}}) →
+  ∀ σ' e',
+    rtc erased_step ([(#();; e (Wrap.lib lib))%E], empty_state) (e', σ') →
+    iterator_trace (trace σ').
+Proof.
+  intros Hlib Hctx σ' e' Hsteps.
+  eapply (@module_invariance Σ _ iterlibN (@iterlib_spec Σ) True e #() (Wrap.lib lib)
+                            iterator_trace empty_state).
+  { cbn. apply iterator_trace_nil. }
+  { iIntros (? ? ?) "?". by iApply Hctx. }
+  { iIntros (? _) "!>". iApply wp_value; eauto. }
+  { iIntros (?). iApply Wrap.correct. iApply Hlib. }
+  eauto.
 Qed.
